plugin/consts.ml
@@ -26,6 +26,7 @@ let cons = resolve "autosubst.list.cons"
 let string = resolve "autosubst.string.type"
 let eq = resolve "autosubst.eq.type"
 let point_eq = resolve "autosubst.point_eq.type"
+let measure_induction = resolve "autosubst.measure_induction"
 
 (**************************************************************************************)
 (** *** Renamings. *)
