plugin/gen_signature.ml
@@ -80,6 +80,9 @@ let generate (s : signature) (ops : ops_zero) : ops_one =
   in
   let mod_O = Names.ModPath.MPdot (mod_T, Names.Label.make "O") in
   (* Build the names of level one constants. *)
+  let const name =
+    Names.Constant.make1 @@ Names.KerName.make mod_O @@ Names.Label.make name
+  in
   let expr =
     (Names.MutInd.make1 @@ Names.KerName.make mod_O @@ Names.Label.make "expr", 0)
   in
@@ -96,5 +99,12 @@ let generate (s : signature) (ops : ops_zero) : ops_one =
   ; e_abase = (expr, 5)
   ; e_aterm = (expr, 6)
   ; e_abind = (expr, 7)
-  ; subst = Names.Constant.make1 @@ Names.KerName.make mod_O @@ Names.Label.make "subst"
+  ; subst = const "subst"
+  ; esize = const "esize"
+  ; inv_Kt = const "inv_Kt"
+  ; inv_Kal_nil = const "inv_Kal_nil"
+  ; inv_Kal_cons = const "inv_Kal_cons"
+  ; inv_Ka_base = const "inv_Ka_base"
+  ; inv_Ka_term = const "inv_Ka_term"
+  ; inv_Ka_bind = const "inv_Ka_bind"
   }
